\documentclass{article}
\usepackage{graphicx}

\begin{document}

\begin{eqnarray*}
  q_i^jf_j &=& \phi f_i\\
  q_i^jg_j &=& \gamma g_i\\
  f^ig_i &=& 0 \\
\\
  Q_{ij}^{kl} &=& 
        q_j^l\delta_i^k + 
        q_i^k\delta_j^l + 
        q_i^k\delta_i^l\delta_j^k +
        q_i^l\delta_i^k\delta_j^l\\
\\
  H_{ij} &=& f_ig_j - g_if_j
\\
  Q_{ij}^{kl}H_{kl} &=& 
                \left(  q_j^l\delta_i^k + 
                        q_i^k\delta_j^l + 
                        q_i^k\delta_i^l\delta_j^k +
                        q_i^l\delta_i^k\delta_j^l\right)
        \cdot  \left(f_kg_l - g_kf_l\right)\\
\\      
  &=& q_j^lf_ig_l - q_j^lg_if_l + q_i^kf_kg_j - q_i^kg_kf_j + 
      q_i^jf_jg_i - q_i^jg_jf_i + q_i^jf_ig_j - q_i^jg_if_j \\
  &=& \gamma f_ig_j - \phi g_if_j + \phi f_ig_j - \gamma g_if_j + 
      \phi f_ig_i - \gamma g_if_i + \gamma f_jg_j - \phi g_jf_j \\
  &=& \left(\gamma + \phi\right)H_{ij}
\end{eqnarray*}


\end{document}
